CollapsingTowers/TwoLevelFull/Examples/StagePower.lean
@@ -1,5 +1,5 @@
 
-import CollapsingTowers.TwoLevelPCP.Typing
+import CollapsingTowers.TwoLevelFull.Typing
 namespace StagePower
 -- stage power function xⁿ
 -- let (power : <ℕ> → ℕ → <ℕ>) =
