CollapsingTowers/TwoLevelFull/Store.lean
@@ -1,0 +1,4 @@
+
+import CollapsingTowers.TwoLevelFull.Syntax
+abbrev Store :=
+  List Expr
