CollapsingTowers/TwoLevelPCP/Examples/Defs.lean
@@ -1,4 +1,0 @@
-
-import CollapsingTowers.TwoLevelPCP.Examples.Counterexamples
-import CollapsingTowers.TwoLevelPCP.Examples.Power
-import CollapsingTowers.TwoLevelPCP.Examples.StagePower
