CollapsingTowers/TwoLevelPCP/Store.lean
@@ -1,4 +1,0 @@
-
-import CollapsingTowers.TwoLevelPCP.Syntax
-abbrev Store :=
-  List Expr
